

**Assignment 2 MLE and MAP (total 20 pts)**  
Student Name: **Komal Wavhal** (Master in Computer Science)  
CWID: **20034443**

1. **Maximum Likelihood estimator** (5 points) Assuming data points are independent and identically distributed (i.i.d.), the probability of the data set given parameters:  $\mu$  and  $\sigma^2$  (the likelihood function):

$$P(\mathbf{x}|\mu, \sigma^2) = \prod_{n=1}^N \mathcal{N}(x_n|\mu, \sigma^2)$$

Please calculate the solution for  $\mu$  and  $\sigma^2$  using Maximum Likelihood (ML) estimator.

**Solution 1:**

**Goal:** Derive closed-form estimators for the mean and variance from the Gaussian likelihood.

Find the values of  $(\mu, \sigma^2)$  that maximize the likelihood  $L(\mu, \sigma^2 | \mathbf{x}_{1:N})$

**Steps-1:** Set up the likelihood and log-likelihood and followed the below steps:

1. Write the log-likelihood  $\ell(\mu, \sigma^2)$  explicitly (keep the constant term; you'll cancel it later).
2. Differentiate  $\ell$  w.r.t.  $\mu$ ; set derivative = 0 and solve.  
*Tip:* the derivative reduces to a sum of residuals  $(x_n - \mu)$ .
3. Differentiate  $\ell$  w.r.t.  $\sigma^2$ ; set = 0 and solve.  
*Tip:* you'll isolate  $\sigma^2$  against a sum of squared residuals.
4. (Optional but strong) **Second-derivative check** (or argue concavity in  $\mu$  and  $\sigma^2$ ) to confirm a maximum.
5. Briefly note the difference between the **MLE variance** (denominator  $N$ ) vs the **unbiased sample variance** (denominator  $N - 1$ ). Examiners like that remark.

Solution

Q. 1

For a normal density

$$N(x | \mu, \sigma^2) = \frac{1}{\sqrt{2\pi\sigma^2}} \exp\left(-\frac{(x-\mu)^2}{2\sigma^2}\right)$$

Assuming independence:

$$L(\mu, \sigma^2 | x_1:N) = \prod_{n=1}^N N(x_n | \mu, \sigma^2)$$

work with the log-likelihood  $l = \log L$ 

$$l(\mu, \sigma^2) = \sum_{n=1}^N \log N(x_n | \mu, \sigma^2)$$

$$= \sum_{n=1}^N \left[ -\frac{1}{2} \log(2\pi\sigma^2) - \frac{(x_n - \mu)^2}{2\sigma^2} \right]$$

$$= -\frac{N}{2} \log(2\pi\sigma^2) - \frac{1}{2\sigma^2} \sum_{n=1}^N (x_n - \mu)^2$$

$$\text{let } S(\mu) = \sum_{n=1}^N (x_n - \mu)^2 \quad \text{to keep notation compact}$$

Differentiate w.r.t  $\mu$ , set to 0, Solve

$$\frac{\partial l}{\partial \mu} = -\frac{1}{\sigma^2} \cdot 2 \sum_{n=1}^N (x_n - \mu)(-1)$$

$$: \left( \frac{\partial}{\partial \mu} = 0 \right) = \frac{1}{\sigma^2} \sum_{n=1}^N (x_n - \mu)$$

Set to zero = 0

$$\sum_{n=1}^N (x_n - \mu) = 0 \quad \mu_{ML} = \bar{x} := \frac{1}{N} \sum_{n=1}^N x_n$$

2nd derivative in  $(\mu)$ 

$$\frac{\partial^2 l}{\partial \mu^2} = \frac{1}{\sigma^2} \sum_{n=1}^N (-1) = -\frac{N}{\sigma^2} < 0$$

So,  $\bar{x}$  gives maximum in  $\mu$

Differentiate w.r.to  $\sigma^2$   
Set to 0, Solve the equation

Treat  $v = \sigma^2$  as the variable  
using the expression above.

$$\ell(\mu, v) = -\frac{N}{2} \log(2\pi v) - \frac{1}{2v} S(\mu)$$

Derivative

$$\frac{\partial \ell}{\partial v} = -\frac{N}{2} \cdot \frac{1}{v} + \frac{1}{2} S(\mu) \cdot \left( \frac{-1}{v^2} \right)$$

with a minus from  $\frac{1}{v} = -\frac{N}{2v} + \frac{S(\mu)}{2v^2}$

Set to zero and multiply by  $2v^2$

$$S(\mu) - Nv = 0$$

$$\Rightarrow \hat{\sigma}^2_{ML} = \frac{1}{N} S(\mu)$$

at the MLE, we plug  $\mu = \hat{\mu} = \bar{x}$ , so

$$\hat{\sigma}^2_{ML} = \frac{1}{N} \sum_{n=1}^N (x_n - \bar{x})^2$$

2nd derivative Check in  $(v = \hat{\sigma}^2)$ :

at the stationary point  $v = \hat{v} = S(\mu)/N$ ,

$$\frac{\partial^2 \ell}{\partial v^2} \Big|_{\hat{v}} = \frac{N}{2} \frac{N^2}{S(\mu)^2} = \frac{S(\mu)}{(S(\mu)/N)^3} = \frac{N^3}{2S(\mu)^2} - \frac{N^3}{S(\mu)^2}$$

$$= -\frac{N^3}{2S(\mu)^2} < 0$$

So, it's a maximum in  $\sigma^2$  as well.

$$\hat{\mu}_{ML} = \bar{x} = \frac{1}{N} \sum_{n=1}^N x_n$$

$$\hat{\sigma}_{ML}^2 = \frac{1}{N} \sum_{n=1}^N (x_n - \bar{x})^2$$

MLE Variance vs. unbiased sample Variance

$$E[\hat{\sigma}_{ML}^2] = \frac{N-1}{N} \sigma^2$$

its a slightly biased low

The unbiased sample variance replaces  $N$  by  $N-1$

$$s^2 := \frac{1}{N-1} \sum_{n=1}^N (x_n - \bar{x})^2 \text{ and } E(s^2) = \sigma^2$$

Sketch of the expectation result - Using the identity

$$\sum_{n=1}^N (x_n - \mu)^2 = \sum_{n=1}^N (x_n - \bar{x} + \bar{x} - \mu)^2 = \sum_{n=1}^N (x_n - \bar{x})^2 + N(\bar{x} - \mu)^2$$

take expectations under  $x_n \stackrel{i.i.d}{\sim} N(\mu, \sigma^2)$

$$\text{recall } E\left[\sum_{n=1}^N (x_n - \mu)^2\right] = N\sigma^2 \text{ and}$$

$$E[(\bar{x} - \mu)^2] = \sigma^2 / N$$

$$\text{This gives } E\left[\sum_{n=1}^N (x_n - \bar{x})^2\right] = (N-1)\sigma^2$$

Let  $x_1, \dots, x_N$  be i.i.d  $\mathcal{N}(\mu, \sigma^2)$  The likelihood and log-likelihood are

$$L(\mu, \sigma^2) = \prod_{n=1}^N \frac{1}{\sqrt{2\pi\sigma^2}} \exp\left(-\frac{(x_n - \mu)^2}{2\sigma^2}\right),$$

$$\ell(\mu, \sigma^2) = \log L = -\frac{N}{2} \log(2\pi\sigma^2) - \frac{1}{2\sigma^2} \sum_{n=1}^N (x_n - \mu)^2$$

Estimate of  $\mu$

$$\frac{\partial \ell}{\partial \mu} = \frac{1}{\sigma^2} \cdot 2 \sum_{n=1}^N (\mu - x_n) = \frac{1}{\sigma^2} \sum_{n=1}^N (x_n - \mu)$$

Set to zero  $\sum_{n=1}^N (x_n - \mu) = 0 \Rightarrow \hat{\mu} = \frac{1}{N} \sum_{n=1}^N x_n$

Second derivative at the optimum:

$$\frac{\partial^2 \ell}{\partial (\sigma^2)^2} = \frac{N}{2(\sigma^2)^3} = \frac{\partial^2 \ell}{\partial (\sigma^2)^3} \quad s = N\sigma^2$$

$$\frac{\partial^2 \ell}{\partial (\sigma^2)^2} = \frac{N}{2(\sigma^2)^3} < 0$$

So, it's maximum

This is MLE variance with denominator  $N$  the unbiased variance uses  $N-1$

$$\hat{\mu}_{ML} = \frac{1}{N} \sum_{n=1}^N x_n \quad \hat{\sigma}_{ML}^2 = \frac{1}{N} \sum_{n=1}^N (x_n - \hat{\mu}_{ML})^2$$

2. **Maximum Likelihood** (5 points) We assume there is a true function  $f(\mathbf{x})$  and the target value is given by  $y = f(x) + \epsilon$  where  $\epsilon$  is a Gaussian distribution with mean 0 and variance  $\sigma^2$ . Thus,

$$p(y|x, w, \beta) = \mathcal{N}(y|f(x), \beta^{-1})$$

where  $\beta^{-1} = \sigma^2$ .

Assuming the data points are drawn independently from the distribution, we obtain the likelihood function:

$$p(\mathbf{y}|\mathbf{x}, w, \beta) = \prod_{n=1}^N \mathcal{N}(y_n|f(x), \beta^{-1})$$

Please show that maximizing the likelihood function is equivalent to minimizing the sum-of-squares error function.

## Solution 2:

**Goal:** Prove that maximizing the likelihood under  $y_n = f(x_n) + \epsilon_n, \epsilon_n \sim \mathcal{N}(0, \beta^{-1})$ , is equivalent to minimizing the **sum of squared errors (SSE)**.

Question 2 Assume  $y_n = f(x_n; w) + \epsilon_n$ ,  
Solution  $\epsilon_n \sim \mathcal{N}(0, \beta^{-1})$   
 So,  
 $p(y_n | x_n, w, \beta) = \mathcal{N}(y_n | f(x_n; w), \beta^{-1})$   
 $= \sqrt{\frac{\beta}{2\pi}} \exp\left(-\frac{\beta}{2} [y_n - f(x_n; w)]^2\right)$   
 $\beta$  (Variance  $\beta^{-1} = \sigma^2$ ) has density  $\sqrt{\beta/2\pi} \exp(-\beta y^2/2)$   
 Assuming sample  $(x_n, y_n)$   
 The likelihood is the product:  

$$L(w, \beta) = \prod_{n=1}^N p(y_n | x_n, w, \beta)$$

$$\left(\frac{\beta}{2\pi}\right)^{N/2} \exp\left(-\frac{\beta}{2} \sum_{n=1}^N [y_n - f(x_n; w)]^2\right)$$
  
 monotone transform:  

$$\ell(w, \beta) = \log L(w, \beta) = \frac{N}{2} \log \beta - \frac{N}{2} \log(2\pi) - \frac{\beta}{2} \sum_{n=1}^N [y_n - f(x_n; w)]^2$$
 let  $SSE(w) := \sum_{n=1}^N [y_n - f(x_n; w)]^2$   
 Then 
$$\ell(w, \beta) = \left[ \frac{N}{2} \log \beta - \frac{N}{2} \log(2\pi) \right] - \frac{\beta}{2} SSE(w)$$
  
 what this reveals that for fixed  $\beta > 0$   
 The only part of  $\ell$  that depends on  $w$  is the term  $-\frac{\beta}{2} SSE(w)$

Argmax of likelihood    Argmin of SSE

for fixed  $\beta > 0$

$$\arg \max_{\omega} l(\omega, \beta) = \arg \max_{\omega} \left[ C - \frac{\beta}{2} \text{SSE}(\omega) \right]$$

$$= \arg \min_{\omega} \text{SSE}(\omega)$$

because adding constant  $C$  doesn't change an argmax, and multiplying by a negative positive constant

here  $-\beta/2$  flips max to min.

$$\arg \max_{\omega} L(\omega, \beta) = \arg \min_{\omega} \sum_{n=1}^N [y_n - f(x_n; \omega)]^2$$

Calculus check:

$$\nabla_{\omega} l(\omega, \beta) = -\frac{\beta}{2} \nabla_{\omega} \text{SSE}(\omega)$$

with  $\beta > 0$  the zeros of  $\nabla_{\omega} l$  are exactly the zeros of  $\nabla_{\omega} \text{SSE}$

maximize over  $\beta$ :

holding  $\omega$  fixed

$$\frac{\partial l}{\partial \beta} = \frac{1}{2\beta} - \frac{1}{2} \frac{\text{SSE}(\omega)}{N}$$

$$\Rightarrow \hat{\beta}_{ML} = \frac{\text{SSE}(\hat{\omega})}{N}$$

This simply picks the precision that matches the residual variance. it doesn't change the fact that  $\hat{\omega}$  minimizes SSE.

Assume  $y_n = f(x_n; \omega) + \epsilon_n$

with  $\epsilon_n \sim \mathcal{N}(y_n | f(x_n; \omega), \beta^{-1})$

$$p(y_n | x_n, \omega, \beta) = \mathcal{N}(y_n | f(x_n; \omega), \beta^{-1})$$

By independence

$$l(\omega) = \prod_{n=1}^N \frac{\sqrt{\beta}}{\sqrt{2\pi}} \exp\left(-\frac{\beta}{2} (y_n - f(x_n; \omega))^2\right)$$

loglikelihood:

$$l(\omega) = \frac{N}{2} \log \beta - \frac{N}{2} \log(2\pi) - \frac{\beta}{2} \sum_{n=1}^N (y_n - f(x_n; \omega))^2$$

$$\text{a.g. } \max_{\omega} l(\omega) = \text{a.g. } \min_{\omega} \sum_{n=1}^N (y_n - f(x_n; \omega))^2$$

So maximizing Gaussian Likelihood is equivalent to maximizing the Sum of Squared errors.

3. **MAP estimator** (5 points) Given input values  $\mathbf{x} = (x_1, \dots, x_N)^T$  and their corresponding target values  $\mathbf{y} = (y_1, \dots, y_N)^T$ , we estimate the target by using function  $f(x, \mathbf{w})$  which is a polynomial curve. Assuming the target variables are drawn from Gaussian distribution:

$$p(y|x, \mathbf{w}, \beta) = \mathcal{N}(y | f(x, \mathbf{w}), \beta^{-1})$$

and a prior Gaussian distribution for  $\mathbf{w}$ :

$$p(\mathbf{w} | \alpha) = \left(\frac{\alpha}{2\pi}\right)^{(M+1)/2} \exp\left(-\frac{\alpha}{2} \mathbf{w}^T \mathbf{w}\right)$$

Please prove that maximum posterior (MAP) is equivalent to minimizing the regularized sum-of-squares error function. Note that the posterior distribution of  $\mathbf{w}$  is  $p(\mathbf{w} | \mathbf{x}, \mathbf{y}, \alpha, \beta)$ . **Hint: use Bayes' theorem.**

### Solution 3:

**Goal:** Show that maximizing the posterior  $p(\mathbf{w} \mid \mathbf{x}, \mathbf{y}, \alpha, \beta)$  is equivalent to minimizing a **regularized** sum of squares with an  $\ell_2$  (weight-decay) term.

### Given:

- Likelihood:  $p(\mathbf{y} \mid \mathbf{x}, \mathbf{w}, \beta) = \mathcal{N}(\mathbf{y} \mid f(\mathbf{x}, \mathbf{w}), \beta^{-1}\mathbf{I})$ .
- Prior:  $p(\mathbf{w} \mid \alpha) \propto \exp\left(-\frac{\alpha}{2} \mathbf{w}^\top \mathbf{w}\right)$ .

### Model (polynomial curve, but any linear-in-parameters model works):

$$f(x; \mathbf{w}) = \boldsymbol{\phi}(x)^\top \mathbf{w}, \quad \boldsymbol{\phi}(x) = [\phi_0(x), \dots, \phi_M(x)]^\top.$$

Stack features into the **design matrix**  $\Phi \in \mathbb{R}^{N \times (M+1)}$  with rows  $\boldsymbol{\phi}(x_n)^\top$ , and labels into  $\mathbf{y} = (y_1, \dots, y_N)^\top$ .

- Likelihood (additive i.i.d. Gaussian noise with precision  $\beta$ ; variance  $\beta^{-1} = \sigma^2$ ):

$$p(\mathbf{y} \mid \mathbf{X}, \mathbf{w}, \beta) = \mathcal{N}(\mathbf{y} \mid \Phi \mathbf{w}, \beta^{-1}\mathbf{I}) = \left(\frac{\beta}{2\pi}\right)^{N/2} \exp\left(-\frac{\beta}{2} \|\mathbf{y} - \Phi \mathbf{w}\|_2^2\right).$$

- Prior on weights (zero-mean isotropic Gaussian with precision  $\alpha$ ):

$$p(\mathbf{w} \mid \alpha) = \left(\frac{\alpha}{2\pi}\right)^{(M+1)/2} \exp\left(-\frac{\alpha}{2} \|\mathbf{w}\|_2^2\right).$$

Using precisions  $\alpha, \beta$  keeps constants clean and makes the posterior exponent a quadratic in  $\mathbf{w}$ , which ensures a Gaussian posterior and a convex optimization.

### Step 1 — Bayes' rule to write the posterior

$$p(\mathbf{w} \mid \mathbf{X}, \mathbf{y}, \alpha, \beta) \propto p(\mathbf{y} \mid \mathbf{X}, \mathbf{w}, \beta) p(\mathbf{w} \mid \alpha).$$

**Why:** MAP maximizes the posterior in  $\mathbf{w}$ . Bayes' rule tells us the posterior is proportional to likelihood times prior; the evidence  $p(\mathbf{y} \mid \mathbf{X}, \alpha, \beta)$  is a constant w.r.t.  $\mathbf{w}$  and can be ignored for the argmax.

Substitute the two densities (drop normalization constants that do not depend on  $\mathbf{w}$ ):

$$p(\mathbf{w} \mid \cdot) \propto \exp\left(-\frac{\beta}{2} \|\mathbf{y} - \Phi \mathbf{w}\|_2^2\right) \exp\left(-\frac{\alpha}{2} \|\mathbf{w}\|_2^2\right) = \exp\left(-\frac{\beta}{2} \|\mathbf{y} - \Phi \mathbf{w}\|_2^2 - \frac{\alpha}{2} \|\mathbf{w}\|_2^2\right).$$

### Step 2 — Take **negative log** posterior

Because  $\log(\cdot)$  is strictly increasing, maximizing the posterior equals minimizing the **negative log-posterior**:

$$\mathcal{L}(\mathbf{w}) := -\log p(\mathbf{w} \mid \mathbf{X}, \mathbf{y}, \alpha, \beta) = \frac{\beta}{2} \|\mathbf{y} - \Phi \mathbf{w}\|_2^2 + \frac{\alpha}{2} \|\mathbf{w}\|_2^2 + \text{const.}$$

### Step 3 — Identify the regularized least-squares objective

Divide by  $\beta/2 > 0$  (a positive scalar doesn't change the minimizer) to obtain:

$$J(\mathbf{w}) = \|\mathbf{y} - \Phi \mathbf{w}\|_2^2 + \lambda \|\mathbf{w}\|_2^2, \quad \lambda = \frac{\alpha}{\beta}.$$

This is exactly **ridge regression** (squared-error loss with  $\ell_2$  weight decay).

Therefore,

$$\mathbf{w}_{\text{MAP}} = \arg \max_{\mathbf{w}} p(\mathbf{w} \mid \mathbf{X}, \mathbf{y}, \alpha, \beta) = \arg \min_{\mathbf{w}} \|\mathbf{y} - \Phi \mathbf{w}\|_2^2 + \lambda \|\mathbf{w}\|_2^2.$$

### This interprets that:

- The likelihood term pushes  $\Phi \mathbf{w}$  to fit the data (small squared residuals).
- The Gaussian prior shrinks weights toward zero;  $\alpha$  controls shrinkage strength.
- $\lambda = \alpha/\beta$  balances fit vs. complexity: larger  $\alpha$  (tighter prior) or smaller  $\beta$  (noisier data)  $\rightarrow$  stronger regularization.

### Step 4 — Closed-form MAP solution

Since  $J(\mathbf{w})$  is a strictly convex quadratic, the unique minimizer satisfies the normal equations:

$$(\Phi^\top \Phi + \lambda \mathbf{I}) \mathbf{w} = \Phi^\top \mathbf{y} \quad \Rightarrow \quad \mathbf{w}_{\text{MAP}} = (\Phi^\top \Phi + \lambda \mathbf{I})^{-1} \Phi^\top \mathbf{y}.$$

Equivalently, in precision form:

$$\mathbf{w}_{\text{MAP}} = (\alpha \mathbf{I} + \beta \Phi^\top \Phi)^{-1} \beta \Phi^\top \mathbf{y}.$$

**Why this form:** It's the minimizer of a positive-definite quadratic; the Hessian is  $\nabla^2 J = 2(\Phi^\top \Phi + \lambda \mathbf{I}) \succ 0$ .

MAP with a zero-mean Gaussian prior on  $\mathbf{w}$  and Gaussian noise is exactly ridge regression:

$$\mathbf{w}_{\text{MAP}} = \arg \min_{\mathbf{w}} \sum_{n=1}^N (y_n - \phi(x_n)^\top \mathbf{w})^2 + \frac{\alpha}{\beta} \|\mathbf{w}\|_2^2.$$

4. **Linear model** (5 points) Consider a linear model of the form:

$$f(\mathbf{x}, \mathbf{w}) = w_0 + \sum_{i=1}^D w_i x_i$$

together with a sum-of-squares error/loss function of the form:

$$L_D(\mathbf{w}) = \frac{1}{2} \sum_{n=1}^N \{f(\mathbf{x}_n, \mathbf{w}) - y_n\}^2$$

Now suppose that Gaussian noise  $\epsilon_i$  with zero mean and variance  $\sigma^2$  is added independently to each of the input variables  $x_i$ . By making use of  $\mathbb{E}[\epsilon_i] = 0$  and  $\mathbb{E}[\epsilon_i \epsilon_j] = \delta_{ij} \sigma^2$  where  $\delta_{ii} = 1$ , show that minimizing  $L_D$  averaged over the noise distribution is equivalent to minimizing the sum-of-squares error for noise-free input variables with the addition of a weight-decay regularization term, in which the bias parameter  $w_0$  is omitted from the regularizer.

#### Solution 4:

**Goal:** With  $f(\mathbf{x}, \mathbf{w}) = w_0 + \sum_{i=1}^D w_i x_i$  and i.i.d. input noise  $x_i \leftarrow x_i + \epsilon_i$ ,  $\mathbb{E}[\epsilon_i] = 0$ ,  $\mathbb{E}[\epsilon_i \epsilon_j] = \delta_{ij} \sigma^2$ , show that minimizing the **expected** loss over the noise is equivalent to minimizing the noiseless SSE **plus** a weight-decay term on  $w_1, \dots, w_D$  (not on  $w_0$ ).

Linear model

$$f(\mathbf{x}, \mathbf{w}) = w_0 + \sum_{i=1}^D w_i x_i$$

$$L_D(\mathbf{w}) = \frac{1}{2} \sum_{n=1}^N (f(\mathbf{x}_n, \mathbf{w}) - y_n)^2.$$

with training loss

disturb **each input coordinate** by independent zero-mean Gaussian noise

$$\tilde{x}_{ni} = x_{ni} + \epsilon_{ni}, \quad \mathbb{E}[\epsilon_{ni}] = 0, \quad \mathbb{E}[\epsilon_{ni} \epsilon_{nj}] = \delta_{ij} \sigma^2,$$

and (implicitly)  $\epsilon_{ni}$  are independent across both  $i$  and  $n$ .

Our goal is to compute  $\mathbb{E}_\epsilon[L_D(\mathbf{w})]$  and show it equals the noiseless data loss plus an  $\ell_2$  penalty on  $w_1, \dots, w_D$ .

## Substitute the noisy inputs

With noise, the prediction on sample  $n$  is

$$f(\tilde{\mathbf{x}}_n, \mathbf{w}) = w_0 + \sum_{i=1}^D w_i (x_{ni} + \varepsilon_{ni}) = \underbrace{\left( w_0 + \sum_{i=1}^D w_i x_{ni} \right)}_{=: a_n} + \sum_{i=1}^D w_i \varepsilon_{ni}.$$

Defined  $a_n = f(\mathbf{x}_n, \mathbf{w})$  as the **noiseless** prediction to separate deterministic and random parts.

## Take expectation over the input noise

Since  $\mathbb{E}[\varepsilon_{ni}] = 0$ ,

$$\mathbb{E} \left[ 2(a_n - y_n) \sum_{i=1}^D w_i \varepsilon_{ni} \right] = 2(a_n - y_n) \sum_{i=1}^D w_i \underbrace{\mathbb{E}[\varepsilon_{ni}]}_0 = 0.$$

The **cross term** vanishes (deterministic factor times zero-mean noise).

For the quadratic noise term, use independence and the given covariance:

$$\begin{aligned} \mathbb{E} \left[ \left( \sum_{i=1}^D w_i \varepsilon_{ni} \right)^2 \right] &= \mathbb{E} \left[ \sum_{i=1}^D \sum_{j=1}^D w_i w_j \varepsilon_{ni} \varepsilon_{nj} \right] \\ &= \sum_{i=1}^D \sum_{j=1}^D w_i w_j \mathbb{E}[\varepsilon_{ni} \varepsilon_{nj}] \\ &= \sum_{i=1}^D w_i^2 \sigma^2 \quad (\text{since } \mathbb{E}[\varepsilon_{ni} \varepsilon_{nj}] = \delta_{ij} \sigma^2). \end{aligned}$$

$$\mathbb{E}_\varepsilon \left[ (f(\tilde{\mathbf{x}}_n, \mathbf{w}) - y_n)^2 \right] = (a_n - y_n)^2 + \sigma^2 \sum_{i=1}^D w_i^2.$$

$$\begin{aligned} \mathbb{E}_\varepsilon [L_D(\mathbf{w})] &= \frac{1}{2} \sum_{n=1}^N \mathbb{E}_\varepsilon \left[ (f(\tilde{\mathbf{x}}_n, \mathbf{w}) - y_n)^2 \right] \\ &= \frac{1}{2} \sum_{n=1}^N (a_n - y_n)^2 + \frac{1}{2} \sum_{n=1}^N \sigma^2 \sum_{i=1}^D w_i^2 \\ &= \underbrace{\frac{1}{2} \sum_{n=1}^N (f(\mathbf{x}_n, \mathbf{w}) - y_n)^2}_{\text{noiseless SSE}} + \underbrace{\frac{N\sigma^2}{2} \sum_{i=1}^D w_i^2}_{\text{weight decay on } w_1, \dots, w_D}. \end{aligned}$$

The bias  $w_0$  **does not appear** in the penalty: the noise perturbs only  $x_i$  (for  $i \geq 1$ ), and  $w_0$  is not multiplied by any  $\varepsilon$ .

The second term is an  $\ell_2$  regularizer with strength

$$\lambda = \frac{N\sigma^2}{2}.$$

Minimizing the expected noisy-input loss is **exactly equivalent** to minimizing, on the **noise-free** inputs, the regularized objective

$$\boxed{\frac{1}{2} \sum_{n=1}^N (f(\mathbf{x}_n, \mathbf{w}) - y_n)^2 + \lambda \sum_{i=1}^D w_i^2} \quad (\text{no penalty on } w_0),$$

with  $\lambda = \frac{N\sigma^2}{2}$  for the total loss (or  $\lambda = \frac{\sigma^2}{2}$  for per-sample average).

**Linear model with input noise & weight decay on non-bias weights**

$$f(\mathbf{x}; w) = w_0 + \sum_{i=1}^D w_i x_i, \quad L_D(w) = \frac{1}{2} \sum_{n=1}^N (f(\mathbf{x}_n; w) - y_n)^2.$$

Suppose inputs are corrupted independently by zero-mean Gaussian noise:

$$\tilde{x}_{ni} = x_{ni} + \varepsilon_{ni}, \quad \mathbb{E}[\varepsilon_{ni}] = 0, \quad \mathbb{E}[\varepsilon_{ni}\varepsilon_{nj}] = \delta_{ij}\sigma^2.$$

We minimize the **expected** loss over the noise:

$$\mathbb{E}[L_D(w)] = \frac{1}{2} \sum_{n=1}^N \mathbb{E} \left[ \left( w_0 + \sum_{i=1}^D w_i \tilde{x}_{ni} - y_n \right)^2 \right].$$

Write  $a_n = w_0 + \sum_i w_i x_{ni} - y_n$  and  $b_n = \sum_i w_i \varepsilon_{ni}$ . Then

$$\mathbb{E}[(a_n + b_n)^2] = a_n^2 + 2a_n\mathbb{E}[b_n] + \mathbb{E}[b_n^2] = a_n^2 + \mathbb{E}[b_n^2],$$

since  $\mathbb{E}[b_n] = \sum_i w_i \mathbb{E}[\varepsilon_{ni}] = 0$ .

Compute the remaining term:

$$\mathbb{E}[b_n^2] = \mathbb{E} \left( \sum_i w_i \varepsilon_{ni} \right)^2 = \sum_{i,j} w_i w_j \mathbb{E}[\varepsilon_{ni}\varepsilon_{nj}] = \sum_{i,j} w_i w_j \delta_{ij} \sigma^2 = \sigma^2 \sum_{i=1}^D w_i^2.$$

Only the weights attached to **noisy inputs** ( $w_1, \dots, w_D$ ) are penalized; the **bias  $w_0$  is not** (it doesn't multiply the noise).

Equivalently, minimizing expected noisy loss is the same (up to a constant factor) as minimizing

$$\mathbb{E}[L_D(w)] = \frac{1}{2} \sum_{n=1}^N a_n^2 + \frac{1}{2} \sum_{n=1}^N \sigma^2 \sum_{i=1}^D w_i^2 = \underbrace{\frac{1}{2} \sum_{n=1}^N (w_0 + \sum_i w_i x_{ni} - y_n)^2}_{\text{noiseless SSE}} + \underbrace{\frac{N\sigma^2}{2} \sum_{i=1}^D w_i^2}_{\text{weight decay}}.$$

**Therefore:**

$$\frac{1}{2} \sum_{n=1}^N (w_0 + \sum_i w_i x_{ni} - y_n)^2 + \lambda \sum_{i=1}^D w_i^2, \quad \lambda = \frac{N\sigma^2}{2} (> 0).$$